backend/ValueAnalysis.v
@@ -1781,7 +1781,7 @@ Lemma alloc_global_match:
   initial_mem_match bc m' (Genv.add_global g idg).
 Proof.
   intros; red; intros. destruct idg as [id1 [fd | gv]]; simpl in *.
-- destruct (Mem.alloc m 0 1) as [m1 b1] eqn:ALLOC.
+- destruct (Mem.alloc_glob id1 m 0 1) as [m1 b1] eqn:ALLOC.
   unfold Genv.find_symbol in H2; simpl in H2.
   unfold Genv.find_var_info, Genv.find_def in H3; simpl in H3.
   rewrite PTree.gsspec in H2. destruct (peq id id1).
@@ -1789,15 +1789,17 @@ Proof.
   assert (sup_In b (Genv.genv_sup g)) by (eapply Genv.genv_symb_range; eauto).
   setoid_rewrite NMap.gso in H3.
   assert (Mem.valid_block m b) by (red; rewrite <- H; auto).
-  assert (b <> b1) by (apply Mem.valid_not_valid_diff with m; eauto with mem).
+  assert (b <> b1). apply Mem.alloc_glob_result in ALLOC.
+  apply Genv.genv_vars_eq in H2. congruence.
   apply bmatch_inv with m.
   eapply H0; eauto.
   intros. transitivity (Mem.loadbytes m1 b ofs n0).
   eapply Mem.loadbytes_drop; eauto.
-  eapply Mem.loadbytes_alloc_unchanged; eauto.
-  intro. rewrite H7 in H6. eapply freshness; eauto.
+  eapply Mem.loadbytes_alloc_glob_unchanged; eauto.
+  apply Genv.genv_vars_eq in H2. congruence.
+  apply Genv.genv_vars_eq in H2. congruence.
 - set (sz := init_data_list_size (gvar_init gv)) in *.
-  destruct (Mem.alloc m 0 sz) as [m1 b1] eqn:ALLOC.
+  destruct (Mem.alloc_glob id1 m 0 sz) as [m1 b1] eqn:ALLOC.
   destruct (store_zeros m1 b1 0 sz) as [m2 | ] eqn:STZ; try discriminate.
   destruct (Genv.store_init_data_list ge m2 b1 0 (gvar_init gv)) as [m3 | ] eqn:SIDL; try discriminate.
   unfold Genv.find_symbol in H2; simpl in H2.
@@ -1806,30 +1808,30 @@ Proof.
 + injection H2; clear H2; intro EQ.
   rewrite EQ in H3. setoid_rewrite NMap.gss in H3. injection H3; clear H3; intros EQ'; subst v.
   assert (b = b1).
-  { erewrite Mem.alloc_result by eauto.
-    rewrite H in EQ. auto. }
+  { erewrite Mem.alloc_glob_result by eauto. congruence. }
   clear EQ. subst b.
   apply bmatch_inv with m3.
   eapply store_init_data_list_sound; eauto.
   apply ablock_init_sound.
   eapply store_zeros_same; eauto.
   split; intros.
-  exploit Mem.load_alloc_same; eauto. intros EQ; subst v; constructor.
-  exploit Mem.loadbytes_alloc_same; eauto with coqlib. congruence.
+  exploit Mem.load_alloc_glob_same; eauto. intros EQ; subst v; constructor.
+  exploit Mem.loadbytes_alloc_glob_same; eauto with coqlib. congruence.
   intros. eapply Mem.loadbytes_drop; eauto.
   right; right; right. unfold Genv.perm_globvar. rewrite H4, H5. constructor.
 + assert (sup_In b (Genv.genv_sup g)) by (eapply Genv.genv_symb_range; eauto).
   setoid_rewrite NMap.gso in H3.
   assert (Mem.valid_block m b) by (red; rewrite <- H; auto).
-  assert (b <> b1) by (apply Mem.valid_not_valid_diff with m; eauto with mem).
+  assert (b <> b1). apply Genv.genv_vars_eq in H2. apply Mem.alloc_glob_result in ALLOC. congruence.
   apply bmatch_inv with m3.
   eapply store_init_data_list_other; eauto.
   eapply store_zeros_other; eauto.
   apply bmatch_inv with m.
   eapply H0; eauto.
-  intros. eapply Mem.loadbytes_alloc_unchanged; eauto.
+  intros. eapply Mem.loadbytes_alloc_glob_unchanged; eauto.
+  apply Mem.alloc_glob_result in ALLOC. congruence.
   intros. eapply Mem.loadbytes_drop; eauto.
-  intro. rewrite H7 in H6. eapply freshness; eauto.
+  apply Genv.genv_vars_eq in H2. congruence.
 Qed.
 
 Lemma alloc_globals_match:
